feat: `Get` `GetSet` `OfFn`, simpNF, notation for `set` (#32)

Algorithm/Data/Classes/AssocArray.lean
@@ -38,11 +38,15 @@ def get (a : Vector α n) (i : Fin n) : α :=
 def set (a : Vector α n) (i : Fin n) (v : α) : Vector α n :=
   ⟨a.1.set (i.cast a.2.symm) v, (Array.size_set _ _ _).trans a.2⟩
 
-lemma get_set (a : Vector α n) (i : Fin n) (v : α) :
-    (a.set i v).get = Function.update a.get i v := by
+lemma get_set_eq (a : Vector α n) (i : Fin n) (v : α) :
+    (a.set i v).get i = v := by
   unfold get set
-  simp_rw [Array.get_fin_set]
-  ext; simp [Function.update, Fin.val_eq_val, eq_comm (a := i)]
+  simp [Array.get_fin_set]
+
+lemma get_set_ne (a : Vector α n) (i : Fin n) (v : α) (j : Fin n) (h : i ≠ j) :
+    (a.set i v).get j = a.get j := by
+  unfold get set
+  simp [Array.get_fin_set, Fin.val_eq_val, h]
 
 @[simp]
 lemma get_ofFn (f : Fin n → α) : (ofFn f).get = f := by
@@ -61,9 +65,38 @@ lemma get_default {f} : (default : Vector.WithDefault α n f).get = f :=
 
 end Batteries793.Vector
 
-class AssocDArray.ReadOnly (C : Type*) (ι : outParam Type*)
-    (α : outParam Type*) (d : outParam <| ι → α) where
+class Get (C : Type*) (ι : outParam Type*) (α : outParam Type*) where
   get : C → ι → α
+
+class GetSet (C : Type*) (ι : outParam Type*) (α : outParam Type*) extends Get C ι α where
+  protected set : C → ι → α → C
+  get_set_eq a i v : get (set a i v) i = v
+  get_set_ne a i v j : i ≠ j → get (set a i v) j = get a j
+export GetSet (get_set_eq get_set_ne)
+
+macro:max a:term noWs "[" i:term " => " v:term "]" : term =>
+  `(GetSet.set $a $i $v)
+
+macro:max a:term noWs "[" i:term " ↦ " v:term "]" : term =>
+  `(GetSet.set $a $i $v)
+
+open Lean PrettyPrinter.Delaborator SubExpr in
+/-- Delaborator for `GetSet.set` -/
+@[delab app.GetSet.set]
+def GetSet.delabSet : Delab := do
+  guard <| (← getExpr).isAppOfArity' ``GetSet.set 7
+  let a ← withNaryArg 4 delab
+  let i ← withNaryArg 5 delab
+  let v ← withNaryArg 6 delab
+  `($a[$i ↦ $v])
+
+class OfFn (C : Type*) (ι : Type*) (α : Type*) [Get C ι α] (f : ι → α) where
+  ofFn : C
+  get_ofFn : Get.get ofFn = f
+export OfFn (ofFn get_ofFn)
+
+class AssocDArray.ReadOnly (C : Type*) (ι : outParam Type*)
+    (α : outParam Type*) (d : outParam <| ι → α) extends Get C ι α where
   toDFinsupp' : C → Π₀' i, [α, d i]
   coe_toDFinsupp'_eq_get : ∀ a : C, ⇑(toDFinsupp' a) = get a
 export AssocDArray.ReadOnly (toDFinsupp' coe_toDFinsupp'_eq_get)
@@ -71,9 +104,8 @@ export AssocDArray.ReadOnly (toDFinsupp' coe_toDFinsupp'_eq_get)
 /-- `AssocDArray C ι α d` is a data structure that acts like a finitely supported function
   `Π₀' i, [α, d i]` with single point update operation. -/
 class AssocDArray (C : Type*) [Inhabited C] (ι : outParam Type*)
-    (α : outParam Type*) (d : outParam <| ι → α) extends AssocDArray.ReadOnly C ι α d where
-  set : C → ι → α → C
-  get_set : [DecidableEq ι] → ∀ a i v, get (set a i v) = Function.update (get a) i v
+    (α : outParam Type*) (d : outParam <| ι → α)
+    extends AssocDArray.ReadOnly C ι α d, GetSet C ι α where
   get_default : get default = d
 
 abbrev AssocArray.ReadOnly (C : Type*) (ι : outParam Type*)
@@ -86,43 +118,85 @@ abbrev AssocArray (C : Type*) [Inhabited C] (ι : outParam Type*)
     (α : outParam Type*) (d : outParam α) :=
   AssocDArray C ι α (fun _ ↦ d)
 
-namespace AssocDArray
+namespace Get
 
-export ReadOnly (get toDFinsupp' coe_toDFinsupp'_eq_get)
+variable {C ι α : Type*}
 
-attribute [simp] get_set get_default coe_toDFinsupp'_eq_get
-
-variable {C ι α : Type*} {d : ι → α}
-
-section ReadOnly
-variable [AssocDArray.ReadOnly C ι α d]
+variable [Get C ι α]
 
 instance : GetElem C ι α fun _ _ ↦ True where
-  getElem a i _ := AssocDArray.get a i
+  getElem a i _ := Get.get a i
 
 @[simp]
 lemma get_eq_getElem (a : C) (i : ι) : get a i = a[i] := rfl
 
-end ReadOnly
+end Get
+
+namespace GetSet
+
+export Get (get)
+
+end GetSet
+
+section GetSet
+open GetSet
+
+variable {C ι α : Type*}
+
+variable [GetSet C ι α]
+
+@[simp]
+lemma getElem_set_eq (a : C) (i : ι) (v : α) :
+    a[i ↦ v][i] = v :=
+  get_set_eq a i v
+
+@[simp]
+lemma getElem_set_ne (a : C) (i : ι) (v : α) (j : ι) (h : i ≠ j) :
+    a[i ↦ v][j] = a[j] :=
+  get_set_ne a i v j h
+
+@[simp]
+lemma getElem_set [DecidableEq ι] (a : C) (i : ι) (v : α) (j : ι) :
+    a[i ↦ v][j] = if i = j then v else a[j] := by
+  split_ifs with h <;> simp [h, getElem_set_eq, getElem_set_ne]
+
+lemma getElem_set_eq_update [DecidableEq ι] (a : C) (i : ι) (v : α) (j : ι) :
+    a[i ↦ v][j] = Function.update (get a) i v j := by
+  simp [Function.update, eq_comm]
+
+lemma get_set [DecidableEq ι] (a : C) (i : ι) (v : α) (j : ι) :
+    get a[i ↦ v] j = if i = j then v else get a j :=
+  getElem_set a i v j
+
+lemma get_set_eq_update [DecidableEq ι] (a : C) (i : ι) (v : α) :
+    get a[i ↦ v] = Function.update (get a) i v :=
+  funext <| getElem_set_eq_update a i v
+
+end GetSet
+
+attribute [simp] AssocDArray.get_default coe_toDFinsupp'_eq_get
+
+section AssocDArray
+
+variable {C ι α : Type*} {d : ι → α}
 
 variable [Inhabited C] [AssocDArray C ι α d]
+
+instance : OfFn C ι α d where
+  ofFn := default
+  get_ofFn := AssocDArray.get_default
 
 lemma toDFinsupp'_apply_eq_getElem (a : C) (i : ι) : toDFinsupp' a i = a[i] := by simp
 
 @[simp]
-lemma getElem_set [DecidableEq ι] (a : C) (i : ι) (v : α) (j : ι) :
-    (set a i v)[j] = Function.update (get a) i v j :=
-  congr_fun (get_set a i v) j
-
-@[simp]
-lemma getElem_default (i : ι) :
+lemma AssocDArray.getElem_default (i : ι) :
     (default : C)[i] = d i :=
-  congr_fun get_default i
+  congr_fun AssocDArray.get_default i
 
 @[simp]
 lemma toDFinsupp'_set [DecidableEq ι] (a : C) (i : ι) (v : α) :
-    toDFinsupp' (set a i v) = (toDFinsupp' a).update i v := by
-  ext; simp
+    toDFinsupp' a[i ↦ v] = (toDFinsupp' a).update i v := by
+  ext; simp [getElem_set_eq_update, -getElem_set]
 
 @[simp]
 lemma toDFinsupp'_default :
@@ -137,7 +211,8 @@ variable {α : Type*} {n : ℕ} {f : Fin n → α}
 instance : AssocDArray (Vector.WithDefault α n f) (Fin n) α f where
   set := set
   get := get
-  get_set a i v := by convert get_set a i v
+  get_set_eq := get_set_eq
+  get_set_ne := get_set_ne
   get_default := get_default
   toDFinsupp' a := DFinsupp'.equivFunOnFintype.symm (get a)
   coe_toDFinsupp'_eq_get _ := DFinsupp'.coe_equivFunOnFintype_symm _
@@ -146,8 +221,8 @@ end Batteries793.Vector
 
 namespace AssocArray
 
-export AssocDArray.ReadOnly (get toDFinsupp' coe_toDFinsupp'_eq_get)
-export AssocDArray (set get_set get_default)
+export Get (get)
+export AssocDArray (get_default)
 
 class Ext (C : Type*) [Inhabited C] (ι : outParam Type*)
     (α : outParam Type*) (d : outParam α) [AssocArray C ι α d] : Prop where
@@ -163,10 +238,11 @@ instance : Inhabited (AssocArray.Quotient C) :=
   inferInstanceAs <| Inhabited (@Quotient C (Setoid.ker get))
 
 instance : AssocArray (AssocArray.Quotient C) ι α d where
-  set q i v := q.map' (set · i v) (by classical exact
-    fun _ _ hm ↦ (Eq.congr (get_set _ _ _) (get_set _ _ _)).mpr (by rw [hm]))
+  set q i v := q.map' (·[i ↦ v]) (by classical exact
+    fun _ _ hm ↦ (Eq.congr (get_set_eq_update _ _ _) (get_set_eq_update _ _ _)).mpr (by rw [hm]))
   get := Quotient.lift get (fun _ _ ↦ id)
-  get_set q i v := q.inductionOn (fun _ ↦ get_set _ _ _)
+  get_set_eq q i v := q.inductionOn (get_set_eq · _ _)
+  get_set_ne q i v j h := q.inductionOn (get_set_ne · _ _ _ h)
   get_default := get_default
   toDFinsupp' := Quotient.lift toDFinsupp' (fun _ _ ↦ by
     simpa only [DFunLike.ext'_iff, coe_toDFinsupp'_eq_get] using id)
@@ -181,8 +257,8 @@ export Ext (ext)
 def listIndicator (l : List ι) (f : ∀ i ∈ l, α) : C :=
   match l with
   | [] => default
-  | (i :: l) => set (listIndicator l (fun i hi ↦ f i (List.mem_cons_of_mem _ hi)))
-    i (f i (List.mem_cons_self _ _))
+  | (i :: l) => (listIndicator l (fun i hi ↦ f i (List.mem_cons_of_mem _ hi)))[i ↦
+    (f i (List.mem_cons_self _ _))]
 
 variable {C}
 
@@ -192,7 +268,7 @@ lemma get_listIndicator [DecidableEq ι] (l : List ι) (f : ∀ i ∈ l, α) :
   | [] => by ext; simp [listIndicator, get_default, Function.const]
   | (i :: l) => by
     ext j
-    rw [listIndicator, get_set, Function.update_apply]
+    rw [listIndicator, get_set_eq_update, Function.update_apply]
     split_ifs with h₁ h₂ h₂
     · simp [h₁]
     · simp [h₁] at h₂
@@ -221,15 +297,11 @@ lemma get_indicator [DecidableEq ι] (s : Finset ι) (f : ∀ i ∈ s, α) :
   rw [get_listIndicator]
   rfl
 
-variable (C)
-
-def ofFn [Fintype ι] (f : ι → α) : C := indicator C Finset.univ (fun i _ ↦ f i)
-
-variable {C}
-
-lemma get_ofFn [DecidableEq ι] [Fintype ι] (f : ι → α) :
-    get (ofFn C f) = f :=
-  (get_indicator _ _).trans <| funext fun _ ↦ dif_pos <| Finset.mem_univ _
+abbrev toOfFn [Fintype ι] (f : ι → α) : OfFn C ι α f where
+  ofFn := indicator C Finset.univ (fun i _ ↦ f i)
+  get_ofFn := by
+    convert (get_indicator _ _).trans <| funext fun _ ↦ dif_pos <| Finset.mem_univ _
+    classical infer_instance
 
 end AssocArray
 
@@ -244,4 +316,4 @@ def DefaultAssocDArray (ι : Type u) (α : Type v) (f : ι → α) {D : Type _} 
 
 instance {n α f} : HasDefaultAssocDArray (Fin n) α f (Batteries793.Vector.WithDefault α n f) where
 
-example {n α f}  := DefaultAssocDArray (Fin n) α f
+example {n α f} := DefaultAssocDArray (Fin n) α f
